src/lib/collections/Collections.Seqs_i.fst
@@ -23,3 +23,30 @@ let reverse_reverse_seq (#a:Type) (s:seq a) :
   Lemma(ensures reverse_seq (reverse_seq s) == s)
   =
   assert (equal (reverse_seq (reverse_seq s)) s)
+
+let rec seq_map_i_indexed (#a:Type) (#b:Type) (f:int->a->b) (s:seq a) (i:int) : 
+  Tot (s':seq b { length s' == length s /\
+                  (forall j . {:pattern index s' j} 0 <= j /\ j < length s ==> index s' j == f (i + j) (index s j))
+                }) 
+      (decreases (length s))
+  =
+  if length s = 0 then createEmpty
+  else cons (f i (head s)) (seq_map_i_indexed f (tail s) (i + 1))
+
+let seq_map_i (#a:Type) (#b:Type) (f:int->a->b) (s:seq a) : 
+  Tot (s':seq b { length s' == length s /\
+                  (forall j . {:pattern index s' j} 0 <= j /\ j < length s ==> index s' j == f j (index s j))
+                })   
+  = 
+  seq_map_i_indexed f s 0
+
+let seq_map_internal_associative (#a:Type) (#b:eqtype) (f:int->a->b) (s:seq a) (pivot:int{0 <= pivot /\ pivot < length s}) :
+  Lemma (let left,right = split s pivot in
+         seq_map_i f s == seq_map_i_indexed f left 0 @| seq_map_i_indexed f right pivot )
+  =
+  let left,right = split s pivot in
+  let full_map = seq_map_i f s in
+  let part1 = seq_map_i_indexed f left 0 in
+  let part2 = seq_map_i_indexed f right pivot in
+  assert (equal (seq_map_i f s) (seq_map_i_indexed f left 0 @| seq_map_i_indexed f right pivot));
+  ()
