src/lib/collections/Collections.Seqs_i.fsti
@@ -15,3 +15,17 @@ val reverse_seq_append (#a:eqtype) (s:seq a) (t:seq a) :
 val reverse_reverse_seq (#a:Type) (s:seq a) : 
   Lemma(ensures reverse_seq (reverse_seq s) == s)
   [SMTPat (reverse_seq (reverse_seq s))]
+
+val seq_map_i_indexed (#a:Type) (#b:Type) (f:int->a->b) (s:seq a) (i:int) : 
+  Tot (s':seq b { length s' == length s /\
+                  (forall j . {:pattern index s' j} 0 <= j /\ j < length s ==> index s' j == f (i + j) (index s j))
+                }) 
+
+val seq_map_i (#a:Type) (#b:Type) (f:int->a->b) (s:seq a) :
+  Tot (s':seq b { length s' == length s /\
+                  (forall j . {:pattern index s' j} 0 <= j /\ j < length s ==> index s' j == f j (index s j))
+                }) 
+
+val seq_map_internal_associative (#a:Type) (#b:eqtype) (f:int->a->b) (s:seq a) (pivot:int{0 <= pivot /\ pivot < length s}) :
+  Lemma (let left,right = split s pivot in
+         seq_map_i f s == seq_map_i_indexed f left 0 @| seq_map_i_indexed f right pivot )
